CIFC.v
@@ -296,6 +296,12 @@ Fixpoint init_field_map (fields : list field) (fm : FieldMap) :=
 
 Check init_field_map.
 
+Record ordinal n := {
+    val :> nat;
+    _   : val < n;
+}.
+
+
 Definition add_heap_obj (h : heap) (o : oid) (ho : heapObj) :=
   fun x' => if beq_oid o x' then (Some ho) else h x'.
 
@@ -328,19 +334,21 @@ Inductive step : tm -> Sigma -> tm -> Sigma -> Prop :=
 
 (* method call *)
   (* context rule: evaluate object target *)
-  | ST_MethodCall1 : forall sigma sigma' e e' id,
+  | ST_MethodCall1 : forall sigma sigma' e e' e2 id,
        e / sigma ==>  e' / sigma' -> 
-      (MethodCall e id e) / sigma ==> (MethodCall e' id e) / sigma'
+      (MethodCall e id e2) / sigma ==> (MethodCall e' id e2) / sigma'
   (* context rule: evaluate arguments *)
-  | ST_MethodCall2 : forall sigma sigma' e e' id t,
-      e <> unlabelOpaque t ->
-       e / sigma ==>  e' / sigma' -> 
-      (MethodCall e id e) / sigma ==> (MethodCall e id e') / sigma'
+  | ST_MethodCall2 : forall sigma sigma' v e e' id,
+      (forall t, value t -> e <> unlabelOpaque t) ->
+      e / sigma ==>  e' / sigma' -> 
+      value v ->
+      (MethodCall v id e) / sigma ==> (MethodCall v id e') / sigma'
   (* normal method call *)
   | ST_MethodCall3 : forall sigma sigma' o s h cls fields v lx l theta s' sf lsf arg_id cls_a body meth returnT,
       sigma = SIGMA s h ->
       Some (Heap_OBJ cls fields lx) = h(o) -> 
       Some (m_def returnT meth cls_a arg_id body) = find_method cls meth -> 
+      value v ->
       sf = sf_update (sf_update empty_stack_frame (Id "this") (ObjId o)) arg_id v ->
       l = (current_label sigma) ->
       lsf = Labeled_frame l sf ->
@@ -351,6 +359,18 @@ Inductive step : tm -> Sigma -> tm -> Sigma -> Prop :=
   (* null pointer exception for method call *)
   | ST_MethodCallException : forall sigma v meth, 
       MethodCall null meth v / sigma ==> NPE / sigma
+
+(* method call with unlabel opaque *)
+  | ST_MethodCall_unlableOpaque : forall sigma sigma' o s h cls fields v lx l' lb s' sf lsf arg_id cls_a body meth returnT,
+      sigma = SIGMA s h ->
+      Some (Heap_OBJ cls fields lx) = h(o) -> 
+      sf = sf_update (sf_update empty_stack_frame (Id "this") (ObjId o)) arg_id v ->
+      l' = join_label lb (current_label sigma) ->
+      lsf = Labeled_frame l' sf ->
+      s' = cons lsf s ->
+      Some (m_def returnT meth cls_a arg_id body) = find_method cls meth ->
+      sigma' = SIGMA s' (get_heap sigma) ->
+      MethodCall (ObjId o) meth (unlabelOpaque ((v_opa_l v (l lb)))) / sigma ==> body / sigma'
 
 (* new expression *)
   | ST_NewExp : forall sigma sigma' F o h cls h' s lb cn f_def m_def,
@@ -375,7 +395,8 @@ Inductive step : tm -> Sigma -> tm -> Sigma -> Prop :=
        e / sigma ==>  e' / sigma' -> 
       (labelData e lb) / sigma ==> (labelData e' lb) / sigma'
   (* label data *)
-  | ST_LabelData2 : forall sigma v_l v lb,
+  | ST_LabelData2 : forall sigma v_l v lb id,
+      (v = ObjId id) ->
       (labelData v lb) / sigma ==> (v_l v lb) / sigma
   (* label data exception *)
   | ST_LabelDataException : forall sigma lb,
@@ -410,6 +431,7 @@ Inductive step : tm -> Sigma -> tm -> Sigma -> Prop :=
   | ST_unlabel_opaque2 : forall sigma v lb l' sigma' s h,
       sigma = SIGMA s h ->
       l' = join_label lb (current_label sigma) ->
+      value (v_opa_l v (l lb)) ->
       (unlabelOpaque ((v_opa_l v (l lb)))) / sigma ==> v / sigma'
 
 (* Opaque call *)
@@ -431,20 +453,10 @@ Inductive step : tm -> Sigma -> tm -> Sigma -> Prop :=
       s = cons lsf s' ->
       lb = (current_label sigma) ->
       sigma' = SIGMA s' h->
+      value v ->
       (opaqueCall (Return v)) / sigma ==> v_opa_l v (l lb) / sigma'
 
-(* method call with unlabel opaque *)
-  | ST_MethodCall_unlableOpaque : forall sigma sigma' o s h cls fields v lx l' lb theta Delta' sf lsf arg_id cls_a body meth returnT,
-      sigma = SIGMA s h ->
-      Some (Heap_OBJ cls fields lx) = h(o) -> 
-      sf = sf_update (sf_update empty_stack_frame (Id "this") (ObjId o)) arg_id v ->
-      l' = join_label lb (current_label sigma) ->
-      lsf = Labeled_frame l' sf ->
-      theta = lsf -> 
-      Delta' = cons theta s ->
-      Some (m_def returnT meth cls_a arg_id body) = find_method cls meth ->
-      sigma' = SIGMA Delta' (get_heap sigma) ->
-      MethodCall (ObjId o) meth (unlabelOpaque ((v_opa_l v (l lb)))) / sigma ==> body / sigma'
+
 
 (* assignment *)
   (* context rule *)
@@ -465,10 +477,11 @@ Inductive step : tm -> Sigma -> tm -> Sigma -> Prop :=
        FieldWrite e1 f e2 / sigma ==> FieldWrite e1' f e2/ sigma'
 
   (* context rule 2 *)
-  | ST_fieldWrite2 : forall sigma sigma' f e1 e2 e2' t,
+  | ST_fieldWrite2 : forall sigma sigma' f v e2 e2' t,
+       value v ->
        e2 <> unlabelOpaque t ->
        e2 / sigma ==>  e2' / sigma' -> 
-       FieldWrite e1 f e2 / sigma ==> FieldWrite e1 f e2'/ sigma'
+       FieldWrite v f e2 / sigma ==> FieldWrite v f e2'/ sigma'
 
   (* field write normal *)
   | ST_fieldWrite3 : forall sigma sigma' o s h h' f lb cls F F' v l',
@@ -514,12 +527,17 @@ Inductive step : tm -> Sigma -> tm -> Sigma -> Prop :=
    (* context rule 2 *)
   | ST_if2 : forall sigma sigma' s1 s2 e2' e2 v, 
        e2 / sigma ==>  e2' / sigma' -> 
+       value v ->
        If v e2 s1 s2 / sigma ==> If v e2' s1 s2 / sigma'
   | ST_if_b1 : forall sigma s1 s2 v1 v2, 
        v1 = v2 ->
+       value v1 ->
+       value v2 ->
        If v1 v2 s1 s2 / sigma ==>  s1 / sigma
   | ST_if_b2 : forall sigma s1 s2 v1 v2, 
        v1 <> v2 ->
+       value v1 ->
+       value v2 ->
        If v1 v2 s1 s2 / sigma ==>  s2 / sigma
 (* sequence *)
    (* context rule *)
@@ -582,7 +600,8 @@ Inductive has_type : Class_table -> typing_context -> heap -> tm -> ty -> Prop :
       arguT = para_T ->
       has_type CT Gamma h (MethodCall e meth argu) (classTy returnT)
 (* new exp *)
-  | T_NewExp : forall h Gamma cn CT,
+  | T_NewExp : forall h Gamma cn CT cls_def,
+      Some cls_def = CT(cn) ->
       has_type CT Gamma h (NewExp cn) (classTy cn)
 (* this *)
   | T_this : forall h Gamma T CT,
@@ -662,113 +681,6 @@ Inductive has_type : Class_table -> typing_context -> heap -> tm -> ty -> Prop :
       has_type CT Gamma h (v_opa_l v lb) (OpaqueLabeledTy T).
 
 
-(*
-Reserved Notation "CT ; h ; Gamma '|-' t '\in' T" (at level 0).
-Inductive has_type : Class_table -> heap -> typing_context -> tm -> ty -> Prop :=
-(*variable *)
-  | T_Var : forall Gamma h x T CT, 
-      Gamma x = Some (classTy T) ->
-      CT ; h ; Gamma |- Tvar x \in (classTy T)
-(* null *)
-  | T_null : forall Gamma h T CT, 
-      CT ; h ; Gamma |- null \in T
-(* Field read *)
-  | T_FieldAccess : forall Gamma e f cls_def CT clsT cls' h,
-      CT ; h ; Gamma |- e \in (classTy clsT) ->
-      Some cls_def = CT(clsT) ->
-      type_of_field (find_fields cls_def) f = Some cls' ->
-      CT ; h ; Gamma |- (FieldAccess e f) \in (classTy cls')
-(* method call *)
-  | T_MethodCall : forall Gamma e meth argu CT h T returnT cls_def body arg_id arguT para_T cls_a,
-      CT ; h ; Gamma |- e \in (classTy T) ->
-      CT ; h ; Gamma |- argu \in arguT ->
-      Some cls_def = CT(T) ->
-      find_method cls_def meth = Some (m_def returnT meth cls_a arg_id body)  ->
-      arguT = para_T ->
-      CT ; h ; Gamma |- MethodCall e meth argu \in (classTy returnT)
-(* new exp *)
-  | T_NewExp : forall h Gamma cn CT,
-      CT ; h; Gamma |- NewExp cn \in (classTy cn)
-(* this *)
-  | T_this : forall h Gamma T CT,
-      CT ; h; Gamma |- this \in T
-(* label *)
-  | T_label : forall h Gamma lb CT,
-      CT ; h ; Gamma |- l lb \in LabelTy
-(* label data *)
-  | T_labelData : forall h Gamma lb CT e T,
-      CT ; h ; Gamma |- lb \in LabelTy ->
-      CT ; h ; Gamma |- e \in T ->
-      CT ; h ; Gamma |- labelData e lb \in (LabelelTy T)
-(* unlabel *)
-  | T_unlabel : forall h Gamma CT e T,
-      CT ; h ; Gamma |- e \in (LabelelTy T) ->
-      CT ; h ; Gamma |- unlabel e \in T
-(* labelOf *)
-  | T_labelOf : forall h Gamma CT e T,
-      CT ; h ; Gamma |- e \in (LabelelTy T) ->
-      CT ; h ; Gamma |- labelOf e \in LabelTy
-(* unlabel opaque *)
-  | T_unlabelOpaque : forall h Gamma CT e T,
-      CT ; h ; Gamma |- e \in (LabelelTy T) -> 
-      CT ; h ; Gamma |- unlabelOpaque e \in T
-(* opaque call *)
-  | T_opaqueCall : forall h Gamma CT e T,
-      CT ; h ; Gamma |- e \in T ->
-      CT ; h ; Gamma |- opaqueCall e \in (OpaqueLabeledTy T)
-(* Skip *)
-  | T_skip : forall h Gamma CT T,
-      CT ; h ; Gamma |- Skip \in T
-(* assignment *)
-  | T_assignment : forall h Gamma CT e T x,
-      Gamma x = Some T ->
-      CT ; h ; Gamma |- e \in T ->
-      CT ; h ; Gamma |- Assignment x e \in T
-(* Field Write *)
-  | T_FieldWrite : forall h Gamma x f cls_def CT clsT cls' e,
-      CT ; h ; Gamma |- x \in (classTy clsT) ->
-      CT ; h ; Gamma |- e \in (classTy cls') ->
-      Some cls_def = CT(clsT) ->
-      type_of_field (find_fields cls_def) f = Some cls' ->
-      CT ; h ; Gamma |- (FieldWrite x f e) \in (classTy cls')
-(* if *)
-  | T_if : forall Gamma h CT e e1 e2 e3 T T',
-      CT ; h ; Gamma |- e \in T ->
-      CT ; h ; Gamma |- e1 \in T ->
-      CT ; h ; Gamma |- e2 \in T' ->
-      CT ; h ; Gamma |- e3 \in T' ->
-      CT ; h ; Gamma |- If e e1 e2 e3 \in T'
-(* sequence *)
-  | T_sequence : forall h Gamma CT e1 e2 T T',
-      CT ; h ; Gamma |- e1 \in T ->
-      CT ; h ; Gamma |- e2 \in T' ->
-      CT ; h ; Gamma |- Sequence e1 e2 \in T'
-(* return *)
-  | T_return : forall h Gamma CT e T,
-      CT ; h ; Gamma |- e \in T ->
-      CT ; h ; Gamma |- Return e \in T
-(* ObjId *)
-  | T_ObjId : forall h Gamma CT o cls_def cls_name,
-      Some cls_def = CT(cls_name) ->
-      CT ; h ; Gamma |- ObjId o \in (classTy cls_name)
-(* NPE *)
-  | T_NPE : forall h Gamma CT T,
-      CT ; h ; Gamma |- NPE \in T
-(* runtime labeled data *)
-  | T_v_l : forall h Gamma lb CT v T,
-      CT ; h ; Gamma |- lb \in LabelTy ->
-      CT ; h ; Gamma |- v \in T ->
-      CT ; h ; Gamma |- v_l v lb \in (LabelelTy T)
-(* runtime labeled data *)
-  | T_v_opa_l : forall h Gamma lb CT v T,
-      CT ; h ; Gamma |- lb \in LabelTy ->
-      CT ; h ; Gamma |- v \in T ->
-      CT ; h ; Gamma |- v_opa_l v lb \in (OpaqueLabeledTy T)
-
-where "CT ; h ; Gamma '|-' t '\in' T" := (has_type CT h Gamma t T).
-*)
-
-
 Definition empty_heap : heap := fun _ => None.
 
 Fixpoint field_lookup (f : id) (fields : list field) :=
@@ -785,6 +697,20 @@ Inductive wfe_fields : (list field) -> FieldMap -> Prop  :=
       fm(x) = Some v ->
       wfe_fields (cons h t) fm.
 
+
+(*
+Inductive wfe_heap : Class_table -> typing_context -> heap -> Prop :=
+  | empty_heap_wfe : forall ct ctx, wfe_heap ct ctx empty_heap
+  | heap_wfe : forall h h' cls_def F cn ct gamma fields newHo o lo,
+        (wfe_heap ct gamma h /\ h(o) = None)
+        -> newHo = Some (Heap_OBJ cls_def F lo)
+        -> Some cls_def  = ct cn
+        -> fields = (find_fields cls_def)
+        -> (forall f cls', type_of_field fields f = Some cls' -> exists v, F(f) = Some v )
+        -> h' = (fun x' => if beq_oid o x' then newHo else h x')
+        -> wfe_heap ct gamma h'.
+*)
+
 Inductive wfe_heap : Class_table -> typing_context -> heap -> Prop :=
   | empty_heap_wfe : forall ct ctx, wfe_heap ct ctx empty_heap
   | heap_wfe : forall h h' o cls_def F cn ct gamma fields ho lo,
@@ -799,15 +725,13 @@ Inductive wfe_heap : Class_table -> typing_context -> heap -> Prop :=
         (*wfe_fields fields F -> *)
         wfe_heap ct gamma h'.
 
+
 Lemma some_eq : forall cls_def F lo cls_def' F' lo',
   Some (Heap_OBJ cls_def F lo) = Some (Heap_OBJ cls_def' F' lo') ->
   cls_def = cls_def' /\ F = F'.
 Proof with auto. 
   intros. inversion H. auto. 
 Qed.  
-
-
-
 
 
 Lemma field_val_of_heap_obj : forall h o gamma CT cls_def F lo cls' fields,
@@ -960,6 +884,33 @@ Definition val_option_type (input : option tm) : tm :=
     | None => null
   end.
 
+Lemma excluded_middle_opaqueLabel : forall e, (exists t, e = unlabelOpaque t) \/ (forall t, ~ (e = unlabelOpaque t)).
+Proof with eauto.
+  intros. case e. 
+right. intro.  intros contra. inversion contra.
+right. intro.  intros contra. inversion contra.
+right. intro.  intros contra. inversion contra.
+right. intro.  intros contra. inversion contra.
+right. intro.  intros contra. inversion contra.
+right. intro.  intros contra. inversion contra.
+right. intro.  intros contra. inversion contra.
+right. intro.  intros contra. inversion contra.
+right. intro.  intros contra. inversion contra.
+right. intro.  intros contra. inversion contra.
+left. exists t. auto. 
+right. intro.  intros contra. inversion contra.
+right. intro.  intros contra. inversion contra.
+right. intro.  intros contra. inversion contra.
+right. intro.  intros contra. inversion contra.
+right. intro.  intros contra. inversion contra.
+right. intro.  intros contra. inversion contra.
+right. intro.  intros contra. inversion contra.
+right. intro.  intros contra. inversion contra.
+right. intro.  intros contra. inversion contra.
+right. intro.  intros contra. inversion contra.
+right. intro.  intros contra. inversion contra.
+Qed.
+
 Theorem progress : forall t T sigma gamma CT s h, 
   sigma = SIGMA s h ->  wfe_heap CT gamma h -> wfe_stack CT gamma h s -> 
   has_type CT gamma h t T -> value t \/ exists t' sigma', t / sigma ==> t' / sigma'.
@@ -1011,36 +962,99 @@ Proof with auto.
     apply ST_fieldRead1 with (sigma:=sigma) (sigma':=sigma') (e:=e) (e':=e') (f:=f). assumption.
 
 (* method call *)
-   -  destruct IHhas_type1. auto. auto. auto. 
+- right.
+   destruct IHhas_type1. auto. auto. auto. 
        + inversion H5. rewrite <- H6 in H2_. inversion H2_.
+          (* case analysis for argument: if the argument is a value *)
+            destruct IHhas_type2. auto. auto. auto. subst. 
+            remember (sf_update (sf_update empty_stack_frame (Id "this") (ObjId o)) arg_id argu) as sf. 
+            remember (SIGMA s h ) as sigma.
+            remember (current_label sigma) as l.
+            remember (Labeled_frame l sf) as lsf. 
+            remember (cons lsf s) as s'.
+            remember (SIGMA s' (get_heap sigma)) as sigma'.
+            exists body. exists sigma'.
+            apply ST_MethodCall3 with (sigma:=sigma) (sigma':=sigma') (o:=o) (s:=s) (h:=h) (cls:=cls_def) (fields:=F) 
+                                       (v:=argu) (lx:=lo) (l:=l) 
+                                       (theta:=lsf) (s':=s') (sf:=sf) (lsf:=lsf) (arg_id:=arg_id) 
+                                        (cls_a:=cls_a) (body:=body) (meth:=meth) (returnT:=returnT); auto.
+            rewrite <- H12 in H2. inversion H2. rewrite <- H13; auto.
+          (* case analysis for argument, if the argument is not a value *)
+            subst. 
+                destruct H14 as [t']. destruct H as [sigma'].
+                pose proof (excluded_middle_opaqueLabel argu).
+                destruct H4.
+                  (* case for argu = unlabelOpaque t *)
+                  destruct H4 as [t]. 
+                  rewrite -> H4 in H. inversion H. subst. 
+                  exists (MethodCall (ObjId o) meth (unlabelOpaque e')).
+                  exists (sigma').
+                  apply ST_MethodCall2 with (sigma:=(SIGMA s h)) (sigma':=sigma') 
+                                            (v:=(ObjId o)) (e:=unlabelOpaque t) (e':=unlabelOpaque e') (id:=meth).
+                  intros. subst. intro contra. inversion contra. rewrite -> H8 in H. inversion H4. 
+                      rewrite <- H6 in H; subst; inversion H7. subst. inversion H7.  subst.  inversion H7.
+                      assumption. apply v_oid. subst. 
+                      remember (SIGMA s h ) as sigma.
+                      remember (sf_update (sf_update empty_stack_frame (Id "this") (ObjId o)) arg_id t') as sf.
+                      remember (join_label lb (current_label sigma)) as l'. 
+                      remember (Labeled_frame l' sf) as lsf. 
+                      remember (cons lsf s) as s'.
+                      remember (SIGMA s' (get_heap sigma)) as sigma''.
+                      exists body. exists sigma''. 
+                      apply ST_MethodCall_unlableOpaque with (sigma:=sigma) (sigma':=sigma'') (o:=o) (s:=s) (h:=h) 
+                                            (cls:=cls_def0) (fields:=F) (v:=t') (lx:=lo) (l':=l') (lb:=lb) (s':=s')
+                                           (sf:=sf) (lsf:=lsf) (arg_id:=arg_id) (cls_a:=cls_a) (body:=body) 
+                                           (meth:=meth) (returnT:=returnT).
+                      auto. auto. auto. auto. auto. auto. subst. 
+                      rewrite <- H12 in H2. inversion H2. rewrite <- H6. rewrite -> H3; auto. 
+                      auto. 
+                  (* case for argu <> unlabelOpaque t *)
+                  exists (MethodCall (ObjId o) meth t'). exists sigma'. 
+                  apply ST_MethodCall2 with (sigma:=(SIGMA s h)) (sigma':=sigma') (v:=((ObjId o))) 
+                                            (e:=argu) (e':=t') (id:=meth).
+                  intro. assert (argu <> unlabelOpaque t). apply (H4 t). intro. assumption. assumption. apply v_oid.
 
-(*
-(* method call *)
-  (* context rule: evaluate object target *)
-  | ST_MethodCall1 : forall sigma sigma' e e' id,
-       e / sigma ==>  e' / sigma' -> 
-      (MethodCall e id e) / sigma ==> (MethodCall e' id e) / sigma'
-  (* context rule: evaluate arguments *)
-  | ST_MethodCall2 : forall sigma sigma' e e' id t,
-      e <> unlabelOpaque t ->
-       e / sigma ==>  e' / sigma' -> 
-      (MethodCall e id e) / sigma ==> (MethodCall e id e') / sigma'
-  (* normal method call *)
-  | ST_MethodCall3 : forall sigma sigma' o s h cls fields v lx l theta s' sf lsf arg_id cls_a body meth returnT,
-      sigma = SIGMA s h ->
-      Some (Heap_OBJ cls fields lx) = h(o) -> 
-      Some (m_def returnT meth cls_a arg_id body) = find_method cls meth -> 
-      sf = sf_update (sf_update empty_stack_frame (Id "this") (ObjId o)) arg_id v ->
-      l = (current_label sigma) ->
-      lsf = Labeled_frame l sf ->
-      theta = lsf -> 
-      s' = cons theta s ->
-      sigma' = SIGMA s' (get_heap sigma) ->
-      MethodCall (ObjId o) meth v / sigma ==> body / sigma'
-  (* null pointer exception for method call *)
-  | ST_MethodCallException : forall sigma v meth, 
-      MethodCall null meth v / sigma ==> NPE / sigma
-*)
+                  subst. exists NPE. exists (SIGMA s h). 
+              apply ST_MethodCallException with (sigma:=(SIGMA s h)) (v:=argu) (meth:=meth).
+
+                  subst. inversion H2_. 
+      +  destruct H5 as [t']. destruct H5 as [sigma']. exists (MethodCall t' meth argu). exists (sigma').   
+                  apply ST_MethodCall1 with (sigma:=sigma) (sigma':=sigma') (e2:=argu) (e:=e) (e':=t') (id:=meth). apply H5.
+
+(* new expression *)
+- right.
+destruct cls_def.
+
+                  
+       | ST_NewExp : forall sigma sigma' F o h cls h' s lb cn f_def m_def,
+      sigma = SIGMA s h->
+      h(o) = None -> 
+      F =  (init_field_map (find_fields cls) empty_field_map) ->
+      lb = (current_label sigma) -> 
+      cls = class_def cn f_def m_def->
+      h' = add_heap_obj h o (Heap_OBJ cls F lb) ->
+      sigma' = SIGMA s h' ->
+      NewExp cn / sigma ==> ObjId o / sigma'              
+                  
+
+
+
+
+
+
+                  apply ST_MethodCall2 with (sigma:=(SIGMA s h)) (sigma':=sigma') 
+                                            (v:=(ObjId o)) (e:=argu) (e':=t') (id:=meth).
+
+
+                  remember (sf_update (sf_update empty_stack_frame (Id "this") (ObjId o)) arg_id argu) as sf. 
+                  
+                  remember (current_label sigma) as l.
+                  remember (Labeled_frame l sf) as lsf. 
+                  remember (cons lsf s) as s'.
+                  remember (SIGMA s' (get_heap sigma)) as sigma'.
+                  exists body. exists sigma'. 
+
+
 
 Theorem preservation : forall t t' T sigma sigma', 
     gamma |- t \in T ->
